more work on checker

deps/poulet4/lib/P4automata/BisimChecker.v
@@ -1,71 +1,92 @@
 Require Import Coq.Relations.Relations.
+Require Import Poulet4.FinType.
 Require Import Poulet4.P4automata.P4automaton.
 Require Import Poulet4.P4automata.PreBisimulationSyntax.
 Require Poulet4.P4automata.WP.
 Import List.ListNotations.
 
 Section BisimChecker.
-  Set Implicit Arguments.
 
   (* State identifiers. *)
   Variable (S: Type).
   Context `{S_eq_dec: EquivDec.EqDec S eq}.
-  Variable (S_elems_replace_w_typeclass: list S).
+  Context `{S_finite: @Finite S _ S_eq_dec}.
 
   (* Header identifiers. *)
   Variable (H: Type).
   Context `{H_eq_dec: EquivDec.EqDec H eq}.
 
   Variable (a: P4A.t S H).
-  Variable (has_extract: forall s H, 0 < P4A.size (a:=a) (exist _ s H)).
 
-  Notation conf := (configuration (P4A.interp a has_extract)).
+  Notation conf := (configuration (P4A.interp a)).
 
-  Notation "⟦ x ⟧" := (interp_crel x).
-  Notation "⦇ x ⦈" := (interp_conf_rel (has_extract:=has_extract) x).
+  Notation "⟦ x ⟧" := (interp_crel a x).
+  Notation "⦇ x ⦈" := (interp_conf_rel a x).
   Notation "R ⊨ q1 q2" := (interp_crel R q1 q2) (at level 40).
   Notation "R ⊨ S" := (forall q1 q2, ⟦R⟧ q1 q2 -> ⦇S⦈ q1 q2) (at level 40).
   Notation δ := step.
 
   Reserved Notation "R ⇝ S" (at level 10).
-  Inductive pre_bisimulation : crel a -> crel a -> relation conf :=
+  Inductive pre_bisimulation : crel S H -> crel S H -> relation conf :=
   | PreBisimulationClose:
       forall R q1 q2,
         ⟦R⟧ q1 q2 ->
         R ⇝ [] q1 q2
   | PreBisimulationSkip:
-      forall (R T: crel a) (C: conf_rel a) q1 q2,
-        R ⇝ T q1 q2 ->
+      forall (R T: crel S H) (C: conf_rel S H) q1 q2,
         R ⊨ C ->
+        R ⇝ T q1 q2 ->
         R ⇝ (C :: T) q1 q2
   | PreBisimulationExtend:
-      forall (R T E: crel a) (C: conf_rel a) q1 q2,
-        (C :: R) ⇝ (T ++ WP.wp C) q1 q2 ->
+      forall (R T: crel S H) (C: conf_rel S H) q1 q2,
+        (C :: R) ⇝ (T ++ WP.wp a C) q1 q2 ->
         R ⇝ (C :: T) q1 q2
   where "R ⇝ S" := (pre_bisimulation R S).
 
-  Definition not_accept1 (s: P4A.state_type a) : conf_rel a := 
+  Definition not_accept1 (s: S) : conf_rel S H := 
     {| cr_st := {| cs_st1 := {| st_state := inr true; st_buf_len := 0 |};
                    cs_st2 := {| st_state := inl s;    st_buf_len := 0 |} |};
        cr_rel := BRFalse _ |}.
 
-  Definition not_accept2 (s: P4A.state_type a) : conf_rel a := 
+  Definition not_accept2 (s: S) : conf_rel S H := 
     {| cr_st := {| cs_st1 := {| st_state := inr true; st_buf_len := 0 |};
                    cs_st2 := {| st_state := inl s;    st_buf_len := 0 |} |};
        cr_rel := BRFalse _ |}.
 
-  Definition init_rel : crel a := 
-    List.map not_accept1 (P4A.list_states a) ++
-    List.map not_accept2 (P4A.list_states a).
+  Definition init_rel : crel S H := 
+    List.map not_accept1 (enum S) ++
+    List.map not_accept2 (enum S).
   
 End BisimChecker.
+Arguments pre_bisimulation {_ _ _ _ _} {_ _} _ _ _.
 
 Require Import Poulet4.P4automata.Examples.
-Definition R0 := init_rel SimpleSplit.aut.
 
+Notation S := (Sum.S Simple.state Split.state).
+Notation H := (Sum.H Simple.header Split.header).
+Notation init_conf := (inl Simple.Start, [], []).
 Lemma prebisim:
-  forall q1 q2,
-    pre_bisimulation (has_extract:=SimpleSplit.has_extract) R0 nil q1 q2.
+  pre_bisimulation Simple.aut nil (init_rel _ _) init_conf init_conf.
 Proof.
+  apply PreBisimulationExtend.
+  simpl.
+  unfold WP.wp, WP.wp_pred_pair, WP.wp_edges, WP.wp_edge, WP.wp_op.
+  simpl.
+  apply PreBisimulationExtend.
+  unfold WP.wp, WP.wp_pred_pair, WP.wp_edges, WP.wp_edge, WP.wp_op.
+  simpl.
+  apply PreBisimulationExtend.
+  unfold WP.wp, WP.wp_pred_pair, WP.wp_edges, WP.wp_edge, WP.wp_op.
+  simpl.
+  apply PreBisimulationSkip; [now intuition|].
+  apply PreBisimulationSkip.
+  {
+    intros.
+    cbn in *.
+    intuition.
+    unfold interp_conf_rel in *; simpl in *.
+    tauto.
+  }
+  apply PreBisimulationClose.
+  cbv.
 Abort.
-       
