deps/poulet4/lib/P4automata/Sum.v
@@ -3,6 +3,7 @@ Import List.ListNotations.
 Require Coq.Logic.Eqdep_dec.
 Require Import Coq.Classes.EquivDec.
 Require Import Coq.Program.Program.
+Require Import Poulet4.FinType.
 Require Import Poulet4.HAList.
 Require Poulet4.P4cub.Envn.
 Require Poulet4.P4cub.BigStep.BSUtil.
@@ -16,8 +17,11 @@ Section Sum.
   (* State identifiers. *)
   Variable (S1: Type).
   Context `{S1_eq_dec: EquivDec.EqDec S1 eq}.
+  Context `{S1_finite: @Finite S1 _ S1_eq_dec}.
+
   Variable (S2: Type).
   Context `{S2_eq_dec: EquivDec.EqDec S2 eq}.
+  Context `{S2_finite: @Finite S2 _ S2_eq_dec}.
 
   (* Header identifiers. *)
   Variable (H1: Type).
@@ -33,12 +37,22 @@ Section Sum.
   Global Instance S_eq_dec: EquivDec.EqDec S eq :=
     ltac:(typeclasses eauto).
 
+  Global Instance S_finite: @Finite S _ S_eq_dec :=
+    ltac:(typeclasses eauto).
+
   Definition H : Type := H1 + H2.
 
   Global Instance H_eq_dec: EquivDec.EqDec H eq :=
     ltac:(typeclasses eauto).
 
-  Definition sum : Syntax.t S H :=
-    Envn.Env.scope_shadow (Syntax.t_fmapSH inl inl a1)
-                          (Syntax.t_fmapSH inr inr a2).
+  Program Definition sum : Syntax.t S H :=
+    {| Syntax.t_states s :=
+         match s with
+         | inl s1 => Syntax.state_fmapSH inl inl (a1.(Syntax.t_states) s1)
+         | inr s2 => Syntax.state_fmapSH inr inr (a2.(Syntax.t_states) s2)
+         end |}.
+  Next Obligation.
+    destruct a1, a2, s;
+      erewrite Syntax.state_fmapSH_size; eauto.
+  Qed.
 End Sum.
